modules/verify/src/main/scala/specrest/verify/z3/Triggers.scala
@@ -11,6 +11,7 @@ object Z3Trigger:
     case Z3Expr.Cmp(_, l, r, _)        => List(l, r)
     case Z3Expr.StrCmp(_, l, r, _)     => List(l, r)
     case Z3Expr.StrConcat(l, r, _)     => List(l, r)
+    case Z3Expr.SeqConcat(l, r, _)     => List(l, r)
     case Z3Expr.Arith(_, args, _)      => args
     case Z3Expr.Quantifier(_, _, b, _) => List(b)
     case Z3Expr.SetLit(_, ms, _)       => ms
